# Linear Ordinal Differential Equations with Constant Coefficients
## Introduction
The equations to be discussed in this chapter are of the form:
$$k_{0}y+k_{1}y'+k_{2}y''+\cdots +k_{n}y^{(n)}=0$$
which may be written in leibniz notation as:
$$k_{0}y+k_{1}\frac{dy}{dx}+k_{2}\frac{d^{2}y}{dx^{2}}+\cdots +k_{n}\frac{d^{n}y}{dx^{n}}=0$$
where $y$ is a function of $x$, but the $k$'s are all constants
These equations are most important in the study of vibrations
of all kinds, mechanical, acoustical, and electrical. This will be
illustrated by the miscellaneous examples at the end of the chapter.
The methods to be given below are chiefly due to Euler and
D'Alembert.*
## First Order Ordinal Differential Equations with Constant Coefficients
The simplest case equations of the first order. If we take $n=1$ the equation becomes
$$k_{0}y+k_{1}\frac{dy}{dx}=0$$
$$k_{1}\frac{dy}{dx}=-k_{0}y$$
$$\frac{1}{y}\frac{dy}{dx}=-\frac{k_{0}}{k_{1}}$$
We can then integrate with respect to $x$
$$\int \frac{1}{y}\frac{dy}{dx}dx=\int -\frac{k_{0}}{k_{1}}dx$$
On the left side we use integration by substitution, while on the right side $-\frac{k_0}{k_1}$ is a constant so we take it out of the integral:
$$ \int\frac{1}{y}dy=-\frac{k_{0}}{k_{1}}\int dx$$
$$ \ln{|y|}+C_1=-\frac{k_{0}}{k_{1}}x+C_2$$
$$ \ln{|y|}=-\frac{k_{0}}{k_{1}}x+C$$
$$ e^{\ln{|y|}}=e^{-\frac{k_{0}}{k_{1}}x+C}$$
$$ |y|=e^{-\frac{k_{0}}{k_{1}}x}e^{C}$$
Because $e$ is a constant, $e^C$ is a constant elevated to another constant, which is just another constant
$$ |y|=Ce^{-\frac{k_{0}}{k_{1}}x}$$
We can move the absolute value on the right:
$$ y=|Ce^{-\frac{k_{0}}{k_{1}}x}|$$
This means:
$$y= 
    \begin{cases}
        Ce^{-\frac{k_{0}}{k_{1}}x}& \text{if } Ce^{-\frac{k_{0}}{k_{1}}x}\geq 0\\
        -Ce^{-\frac{k_{0}}{k_{1}}x}& \text{if } Ce^{-\frac{k_{0}}{k_{1}}x} < 0
    \end{cases}
$$
But being negative just means being multiplied by $-1$ which is a constant, by the same line of reasoning as before then, we can write our solution as
$$ y=Ce^{-\frac{k_{0}}{k_{1}}x}$$
## Second Order Ordinal Differential Equations with Constant Coefficients
If we take $n=2$ the equation becomes:
$$k_{0}y+k_{1}\frac{dy}{dx}+k_2\frac{d^2y}{dx^2}=0$$
The solution of the first order equation suggests that a solution for this one could be of the form $y = Ce^{tx}$, where m is a constant.  
If that was the case, than the derivatives of $y$ would be:
$$\frac{dy}{dx} = tCe^{tx}$$
$$\frac{d^2y}{dx^2} = t^2Ce^{tx}$$
So if we substitute in the equation:
$$k_{0}Ce^{tx}+k_{1}tCe^{tx}+k_2m^2Ce^{tx}=0$$
And we factor out $Ce^{tx}$:
$$Ce^{tx}(k_{0}+k_{1}t+k_2t^2)=0$$
It becomes clear that the only case in which the left side of the equation is equal to $0$ is if the polynomial of $m$ inside the parenthesis is equal to $0$, this means that we have to find a value for $m$ that makes that polinomyal equal to $0$, in other words we have to find the roots of the polinomyal, the problem of solving a differential equation of 2nd order differential equation has turned into having to solve a 2nd grade equation. To simbolyze this symilarity we call the plynomial *characteristic polynomial* and the equation that is generated by posing it equal to $0$ *characteristic equation*.  
The soulution depends on the discriminant of the charateristic equation:
$$\Delta=k_1^2-4k_2k_1$$
### Positive Discriminant
If the $\Delta$ is positive then there are two different solution to the charateristic equation, if we call them $a$ and $b$, then the solutions of the differential equation can be written out as:  
$y=C_1e^{a x}$ and $y=C_2e^{b x}$  
There is an interesting property of this equation, which can be found by taking $C_1e^{a x}+C_2e^{b x}$ as a solution, in fact if we substitute back into the original equation:
$$k_{0}(C_1e^{a x}+C_2e^{b x})+k_{1}(a C_1e^{a x}+b C_2e^{b x})+k_2(a^2C_1e^{a x}+b^2C_2e^{b x})=0$$
$$k_{0}C_1e^{a x}+k_{0}C_2e^{b x}+k_{1}a C_1e^{a x}+k_{1}b C_2e^{b x}+k_2a^2C_1e^{a x}+k_2b^2C_2e^{b x}=0$$
$$C_1e^{a x}(k_{0}+k_{1}a+k_2a^2)+C_2e^{b x}(k_{0}+k_{1}b+k_2b^2)=0$$
by definition $a$ and $b$ are solutions respectively to the first and second charateristic polinomyals, this means that the left side of the equation simplifies to $0$ and $C_1e^{a x}+C_2e^{b x}$ is in fact a solution to the differential equation. This could have been suggested by the fact that the equation is *linear*.  
As this third solution contains two arbitrary constants, equal in number to the order of the equation, we shall regard it as the general solution.
### Zero Discriminant
if the $\Delta$ is equal to $0$, then the charateristic equation has equal solutions $a = b$, and the solution
$$y=C_1e^{a x}+C_2e^{b x}$$
reduces to
$$y=(C_1+C_2)e^{a x}=(C_1+C_2)e^{b x}$$
but $C_1+C_2$, the sum of two arbitrary constant, is really only a single arbitrary constant. Because we have seen the solution of a differential equation must have the same number of constants as the order of the differential equation, this solution cannot be regarded as the most general one.  

To found a more general one, one thing you could think of would be to take $y=Ce^{a x}V=Ce^{b x}V$, where $V$ is a function of $x$.
Also if we know that the charateristic equation has $a=b$ as a solution,then we can rewrite it from:
$$(t-a)(t-b)=0$$
to:
$$(t-a)(t-a)=0$$
$$t^2-2at+a^2=0$$
The original differential equation will then become:
$$a^2y-2a\frac{dy}{dx}+\frac{d^2y}{dx^2}=0$$
If we apply the power rule:
$$\frac{d}{dx}(uv)=v\frac {du}{dx}+u\frac {dv}{dx}$$
To calculate the derivative of $y=Ce^{a x}V$, where $u=e^{a x}$ and $v=V$
$$\frac{dy}{dx}=C\frac{d}{dx}(e^{a x}V)$$
$$\frac{dy}{dx}=C\left(Va e^{a x}+e^{a x}\frac{dV}{dx}\right)$$
$$\frac{dy}{dx}=Ce^{a x}\left(Va +\frac{dV}{dx}\right)$$
And we repeat this tedious process for the second derivative by derivating the first one:
$$\frac{d^2y}{dx^2}=C\frac{d}{dx}\left(Va e^{a x}+e^{a x}\frac{dV}{dx}\right)$$
$$\frac{d^2y}{dx^2}=C\left(a^2 e^{a x}V+a e^{a x}\frac{dV}{dx}+a e^{a x}\frac{dV}{dx}+e^{a x}\frac{d^2V}{dx^2}\right)$$
$$\frac{d^2y}{dx^2}=C\left(a^2 e^{a x}V+2a e^{a x}\frac{dV}{dx}+e^{a x}\frac{d^2V}{dx^2}\right)$$
$$\frac{d^2y}{dx^2}=Ce^{a x}\left(a^2 V+2a\frac{dV}{dx}+\frac{d^2V}{dx^2}\right)$$
We are now "only" left with substituting back into the differential equation:
$$a^2Ce^{a x}V-2a Ce^{a x}\left(Va +\frac{dV}{dx}\right)+Ce^{a x}\left(a^2 V+2a\frac{dV}{dx}+\frac{d^2V}{dx^2}\right)=0$$
$$Ce^{a x}\left(a^2 V\right)+Ce^{a x}\left(-2a^2 V-2a\frac{dV}{dx}\right)+Ce^{a x}\left(a^2 V+2a\frac{dV}{dx}+\frac{d^2V}{dx^2}\right)=0$$
$$Ce^{a x}\left(a^2 V-2a^2 V-2a\frac{dV}{dx}+a^2 V+2a\frac{dV}{dx}+\frac{d^2V}{dx^2}\right)=0$$
$$Ce^{a x}\left(\frac{d^2V}{dx^2}\right)=0$$
As before, the exponential cannot be $0$, so the only thing that can make the equation true is the second derivative of $V$ being equal to $0$:
$$\frac{d^2V}{dx^2}=0$$
$$\int\frac{d^2V}{dx^2}dx=\int0dx$$
$$\frac{dV}{dx}=C_1$$
$$\int\frac{dV}{dx}dx=\int C_1dx$$
$$V=C_1x+C_2$$
By substituting back into the initial supposed solution $V$, we have found a general solution for $\Delta = 0$ that satisfies the condition of having two arbitrary constants:
$$y=e^{a x}(C_1x+C_2)$$
### Negative Discriminant
If $\Delta$ is negative then the charateristic equation has two complex solutions, namely:
$$a=\alpha +i\beta $$
$$b=\alpha -i\beta $$
And the solution to the differential equation becomes:
$$y=C_1e^{(\alpha +i\beta )x}+C_2e^{(\alpha -i\beta )x}$$
but we could want a solution that is completely real, we can obtain one with Euler's formula:
$$e^{ix}=\cos(x)+i\sin(x)$$
by subdividing the $e$'s and substituting:
$$y=C_1e^{\alpha x+i\beta x}+C_2e^{\alpha x-i\beta x}$$
$$y=C_1e^{\alpha x}e^{i\beta x}+C_2e^{\alpha x}e^{-i\beta x}$$
$$y=C_1e^{\alpha x}(\cos(i\beta x)+i\sin(i\beta x))+C_2e^{\alpha x}(\cos(-i\beta x)+i\sin(-i\beta x))$$
$$y=e^{\alpha x}(C_1\cos(i\beta x)+iC_1\sin(i\beta x)+C_2\cos(-i\beta x)+iC_2\sin(-i\beta x))$$
Because of the fact that sine is an odd function and cosine is an even function:
$$\sin(-x)=-\sin(x)$$
$$\cos(-x)=\cos(x)$$
We can rewrite as:
$$y=e^{\alpha x}(C_1\cos(\beta x)+iC_1\sin(\beta x)+C_2\cos(\beta x)-iC_2\sin(\beta x))$$
$$y=e^{\alpha x}((C_1+C_2)(2\cos(\beta x))+i(C_1-C_2)(2\sin(\beta x)))$$
$$y=e^{\alpha x}(C_3\cos(\beta x)+C_4\sin(\beta x))$$
Where $C_3=2(C_1+C_2)$ and $C_4=2(C_1-C_2)$. At first sight it may seem as if $C_4$ must be imaginary, but it isn't really necessary




